src/NLustre/NLustre.v
@@ -27,17 +27,17 @@ Module Type NLUSTRE
        (CE    : COREEXPR Ids   Op OpAux IStr).
   Declare Module Export Syn        : NLSYNTAX             Ids Op       CE.Syn.
   Declare Module Export Ord        : NLORDERED            Ids Op       CE.Syn Syn.
-  Declare Module Export Norm       : NLNORMALARGS         Ids Op       CE.Syn Syn.
   Declare Module Export IsF        : ISFREE               Ids Op       CE.Syn Syn CE.IsF.
   Declare Module Export CoindSem   : NLCOINDSEMANTICS     Ids Op OpAux CE.Syn Syn CStr Ord.
   Declare Module Export Sem        : NLINDEXEDSEMANTICS   Ids Op OpAux CE.Syn Syn IStr Ord CE.Sem.
   Declare Module Export CoindToIdx : NLCOINDTOINDEXED     Ids Op OpAux CE.Syn Syn IStr CStr Ord CE.Sem Sem CoindSem.
-  Declare Module Export Typ        : NLTYPING             Ids Op       CE.Syn Syn     Ord CE.Typ.
+  Declare Module Export Typ        : NLTYPING             Ids Op       CE.Syn Syn      Ord CE.Typ.
+  Declare Module Export Norm       : NLNORMALARGS         Ids Op       CE.Syn CE.Typ Syn Ord Typ.
   Declare Module Export Mem        : MEMORIES             Ids Op       CE.Syn Syn.
   Declare Module Export IsD        : ISDEFINED            Ids Op       CE.Syn Syn                     Mem.
   Declare Module Export IsV        : ISVARIABLE           Ids Op       CE.Syn Syn                     Mem IsD.
   Declare Module Export NoD        : NODUP                Ids Op       CE.Syn Syn                     Mem IsD IsV.
-  Declare Module Export Clo        : NLCLOCKING           Ids Op       CE.Syn Syn     Ord             Mem IsD CE.IsF IsF CE.Clo.
+  Declare Module Export Clo        : NLCLOCKING           Ids Op       CE.Syn Syn      Ord             Mem IsD CE.IsF IsF CE.Clo.
   Declare Module Export CloSem     : NLCLOCKINGSEMANTICS  Ids Op OpAux CE.Syn Syn IStr Ord CE.Sem Sem Mem IsD CE.IsF IsF CE.Clo Clo CE.CloSem.
   Declare Module Export MemSem     : NLMEMSEMANTICS       Ids Op OpAux CE.Syn Syn IStr Ord CE.Sem Sem Mem IsD IsV CE.IsF IsF NoD CE.Clo Clo CE.CloSem CloSem.
 End NLUSTRE.
@@ -52,12 +52,12 @@ Module NLustreFun
 <: NLUSTRE Ids Op OpAux CStr IStr CE.
   Module Export Syn        := NLSyntaxFun             Ids Op       CE.Syn.
   Module Export Ord        := NLOrderedFun            Ids Op       CE.Syn Syn.
-  Module Export Norm       := NLNormalArgsFun         Ids Op       CE.Syn Syn.
   Module Export IsF        := IsFreeFun               Ids Op       CE.Syn Syn CE.IsF.
   Module Export CoindSem   := NLCoindSemanticsFun     Ids Op OpAux CE.Syn Syn CStr Ord.
   Module Export Sem        := NLIndexedSemanticsFun   Ids Op OpAux CE.Syn Syn IStr Ord CE.Sem.
   Module Export CoindToIdx := NLCoindToIndexedFun     Ids Op OpAux CE.Syn Syn IStr CStr Ord CE.Sem Sem CoindSem.
   Module Export Typ        := NLTypingFun             Ids Op       CE.Syn Syn     Ord CE.Typ.
+  Module Export Norm       := NLNormalArgsFun         Ids Op       CE.Syn CE.Typ Syn Ord Typ.
   Module Export Mem        := MemoriesFun             Ids Op       CE.Syn Syn.
   Module Export IsD        := IsDefinedFun            Ids Op       CE.Syn Syn                     Mem.
   Module Export IsV        := IsVariableFun           Ids Op       CE.Syn Syn                     Mem IsD.
